#Fold-Right and Fold-Left

```Scheme
>(fold-right / 1 (list 1 2 3))
3/2

>(fold-left  / 1 (list 1 2 3))
1/6

>(fold-right list nil (list 1 2 3))
(1 (2 (3 ())))

>(fold-left  list nil (list 1 2 3))
(((() 1) 2) 3)
```

It might be confusing at first. Let's expand the first two expressions.

1. 1 = 1 => 3 / 1 = 3 => 2 / 3 = 2/3 => 1 / 2/3 = 3/2
2. 1 = 1 => 1 / 1 = 1 => 1 / 2 = 1/2 => 1/2 / 3 = 1/6

Two distinctions:

1. ``fold-right`` extracts values from sequence in a right-to-left order while
``fold-left`` does in a left-to-right order.
2. ``fold-right``'s (op this last) versus ``fold-left``'s (op last this)

If (op p1 p2) is equivalent to (op p2 p1), same results would be produced using
both procedures.

```Scheme
>(fold-right * 1 (list 1 2 3))
6

>(fold-left * 1 (list 1 2 3))
6
```
